array as function

Array.thy
@@ -7,37 +7,20 @@ type_synonym 'a array = "nat \<Rightarrow> 'a"
 definition interval :: "nat \<Rightarrow> nat \<Rightarrow> nat set" where
   "interval k l \<equiv> {i. k \<le> i \<and> i \<le> l}"
 
-abbreviation array_length :: "'a array \<Rightarrow> nat" ("len _" [999] 1000) where
-  "len a \<equiv> snd a"
+(* Sum from offset the number of value n *)
+primrec array_sum :: "nat \<Rightarrow> nat \<Rightarrow> 'a array \<Rightarrow> 'a :: {plus, zero}" where
+  "array_sum off 0 a = 0"
+| "array_sum off (Suc n) a = a (off + n) + array_sum off n a"
 
-definition array_at :: "'a array \<Rightarrow> nat \<Rightarrow> 'a" (infixl "at" 100) where
-  "a at i \<equiv> fst a i"
+fun array_sorted :: "nat \<Rightarrow> nat \<Rightarrow> 'a :: order array \<Rightarrow> bool" where
+  "array_sorted off 0 a \<longleftrightarrow> True"
+| "array_sorted off (Suc 0) a \<longleftrightarrow> True" 
+| "array_sorted off (Suc (Suc n)) a \<longleftrightarrow> a (off + n) \<le> a (off + Suc n) \<and> array_sorted off (Suc n) a"
 
-definition array_update :: "'a array \<Rightarrow> nat \<Rightarrow> 'a \<Rightarrow> 'a array" where
-  "array_update a i n \<equiv> ((fst a) (i := n), snd a)"
+fun new_array :: "'a list \<Rightarrow> 'a array" where
+  "new_array xs = nth xs"
 
-fun array_fold :: "('a \<Rightarrow> 'b \<Rightarrow> 'b) \<Rightarrow> 'a array \<Rightarrow> 'b \<Rightarrow> 'b" where
-  "array_fold f (a, 0) = id"
-| "array_fold f (a, Suc n) = array_fold f (a, n) o f (a (Suc n))"
-
-fun array_foldl :: "('b \<Rightarrow> 'a \<Rightarrow> 'b) \<Rightarrow> 'b \<Rightarrow> 'a array \<Rightarrow> 'b" where
-  "array_foldl f b (a, 0) = b"
-| "array_foldl f b (a, Suc n) = array_foldl f (f b (a (Suc n))) (a, n)"
-
-primrec new_array_acc :: "'a list \<Rightarrow> (nat \<Rightarrow> 'a ) \<Rightarrow> nat \<Rightarrow> nat \<Rightarrow> 'a" where
-  "new_array_acc (x#xs) f n = new_array_acc xs (f(n := x)) (Suc n)"
-| "new_array_acc [] f n = f"
-
-definition new_array_list :: "'a list \<Rightarrow> 'a array" where
-  "new_array_list xs \<equiv> (new_array_acc xs (\<lambda>_. SOME n. True) 1, length xs + 1)"
-
-fun sum_from_to :: "nat \<Rightarrow> nat \<Rightarrow> ('a :: {plus, zero}) array \<Rightarrow> 'a" where
-  "sum_from_to i 0 a = 0"
-| "sum_from_to i (Suc j) a = (if i \<le> Suc j then sum_from_to i j a + a at (Suc j) else 0)"
-
-definition sum :: "('a :: {plus, zero}) array \<Rightarrow> 'a" where
-  "sum a \<equiv> sum_from_to 1 (len a) a"
+value "array_sorted 1 3 (new_array [0, 5, 8 :: nat, 4])"
 
 
-value "sorted_from_to 2 4 (new_array_list [1, 2, 3 :: nat, 4, 5])"
 end
